Add solution for Pset10

pset10/Pset10.v
@@ -9,6 +9,9 @@ Require Import Frap.
 
 Set Implicit Arguments.
 
+Ltac elimc var := elim var; clear var.
+Ltac pinvert expr := pose (pinvert_tmp := expr); invert pinvert_tmp.
+
 (** * Hoare Logic with Input/Output Traces *)
 
 (* Hoare logic as covered in lecture is only the beginning, so far as
@@ -146,9 +149,66 @@ Open Scope reset_scope.
 
 (** * Define your semantics here! *)
 
-Axiom exec : trace -> heap -> valuation -> cmd ->
-             trace -> heap -> valuation -> Prop.
+Fixpoint interp (e : exp) (h: heap) (v : valuation) : nat :=
+  match e with
+  | Const n => n
+  | Var x =>
+    match v $? x with
+    | None => 0
+    | Some n => n
+    end
+  | Read e1 =>
+    match h $? (interp e1 h v) with
+    | None => 0
+    | Some n => n
+    end
+  | Plus e1 e2 => interp e1 h v + interp e2 h v
+  | Minus e1 e2 => interp e1 h v - interp e2 h v
+  | Mult e1 e2 => interp e1 h v * interp e2 h v
+  end.
 
+Definition interpb (be: bexp) (h: heap) (v : valuation) : bool :=
+  match be with
+  | Equal e1 e2 => if interp e1 h v ==n interp e2 h v then true else false
+  | Less e1 e2 => if lt_dec (interp e1 h v) (interp e2 h v) then true else false
+  end.
+
+Inductive exec : trace -> heap -> valuation -> cmd ->
+                 trace -> heap -> valuation -> Prop :=
+  | ExecSkip : forall t h v, exec t h v Skip t h v
+  | ExecAssign : forall t h v x e,
+    exec t h v (Assign x e) t h (v $+ (x, interp e h v))
+  | ExecWrite : forall t h v e1 e2,
+    exec t h v (Write e1 e2) t (h $+ (interp e1 h v, interp e2 h v)) v
+  | ExecSeq : forall t1 h1 v1 c1 t2 h2 v2 c2 t3 h3 v3,
+    exec t1 h1 v1 c1 t2 h2 v2 ->
+    exec t2 h2 v2 c2 t3 h3 v3 ->
+    exec t1 h1 v1 (Seq c1 c2) t3 h3 v3
+  | ExecIfTrue : forall t1 h1 v1 be then_ else_ t2 h2 v2,
+    interpb be h1 v1 = true ->
+    exec t1 h1 v1 then_ t2 h2 v2 ->
+    exec t1 h1 v1 (If_ be then_ else_) t2 h2 v2
+  | ExecIfFalse : forall t1 h1 v1 be then_ else_ t2 h2 v2,
+    interpb be h1 v1 = false ->
+    exec t1 h1 v1 else_ t2 h2 v2 ->
+    exec t1 h1 v1 (If_ be then_ else_) t2 h2 v2
+  | ExecWhileTrue : forall t1 h1 v1 (inv: assertion) be body t2 h2 v2 t3 h3 v3,
+    inv t1 h1 v1 ->
+    interpb be h1 v1 = true ->
+    exec t1 h1 v1 body t2 h2 v2 ->
+    exec t2 h2 v2 (While_ inv be body) t3 h3 v3 ->
+    exec t1 h1 v1 (While_ inv be body) t3 h3 v3
+  | ExecWhileFalse : forall t h v (inv: assertion) be body,
+    inv t h v ->
+    interpb be h v = false ->
+    exec t h v (While_ inv be body) t h v
+  | ExecAssert : forall t h v (a: iassertion),
+    a h v ->
+    exec t h v (Assert a) t h v
+  | ExecInput : forall t h v x n,
+    exec t h v (Input x) ((In n)::t) h (v $+ (x, n))
+  | ExecOutput : forall t h v e,
+    exec t h v (Output e) ((Out (interp e h v))::t) h v.
 
 (** * Task 2 : Hoare logic *)
 
@@ -166,13 +226,57 @@ Axiom exec : trace -> heap -> valuation -> cmd ->
 
 (** Task 2-1: Define your Hoare logic here! *)
 
-Axiom hoare_triple : assertion -> cmd -> assertion -> Prop.
-
 Notation "[[ tr , h , v ]] ~> e" := (fun tr h v => e%reset) (at level 90).
+
+Inductive hoare_triple : assertion -> cmd -> assertion -> Prop :=
+  | HoareSkip : forall P, hoare_triple P Skip P
+  | HoareAssign : forall P x e,
+    hoare_triple P (Assign x e) ([[t, h, v]] ~>
+        exists v', P t h v' /\ v = v' $+ (x, interp e h v'))
+  | HoareWrite : forall P e1 e2,
+    hoare_triple P (Write e1 e2) ([[t, h, v]] ~>
+        exists h', P t h' v /\ h = h' $+ (interp e1 h' v, interp e2 h' v))
+  | HoareSeq : forall P e1 Q e2 R,
+    hoare_triple P e1 Q -> hoare_triple Q e2 R ->
+    hoare_triple P (Seq e1 e2) R
+  | HoareIf : forall P eb then_ Q1 else_ Q2,
+    hoare_triple ([[t, h, v]] ~> P t h v /\ interpb eb h v = true) then_ Q1 ->
+    hoare_triple ([[t, h, v]] ~> P t h v /\ interpb eb h v = false) else_ Q2 ->
+    hoare_triple P (If_ eb then_ else_) ([[t, h, v]] ~> Q1 t h v \/ Q2 t h v)
+  | HoareWhile : forall (P I: assertion) be body,
+    (forall t h v, P t h v -> I t h v) ->
+    hoare_triple ([[t, h, v]] ~> I t h v /\ interpb be h v = true) body I ->
+    hoare_triple P (While_ I be body) ([[t, h, v]] ~>
+        I t h v /\ interpb be h v = false)
+  | HoareAssert : forall (P: assertion) (I: iassertion),
+    (forall t h v, P t h v -> I h v) ->
+    hoare_triple P (Assert I) P
+  | HoareInput : forall P x,
+    hoare_triple P (Input x) ([[t, h, v]] ~>
+        exists t' v' n, P t' h v' /\ v = v' $+ (x, n) /\ t = (In n)::t')
+  | HoareOutput : forall P e,
+    hoare_triple P (Output e) ([[t, h, v]] ~>
+        exists t', P t' h v /\ t = (Out (interp e h v))::t')
+  | HoareConseq : forall c (P P' Q Q': assertion),
+    hoare_triple P c Q ->
+    (forall t h v, P' t h v -> P t h v) ->
+    (forall t h v, Q t h v -> Q' t h v) ->
+    hoare_triple P' c Q'.
+
 Notation "{{ P }} c {{ Q }}" :=
   (hoare_triple P c%cmd Q) (at level 90, c at next level).
 
 (** Task 2-2: Prove the consistency theorem. *)
+
+Lemma hoare_while : forall t1 h1 v1 inv be body t2 h2 v2,
+    exec t1 h1 v1 (While_ inv be body) t2 h2 v2 ->
+    inv t2 h2 v2 /\ interpb be h2 v2 = false.
+Proof.
+  simplify.
+  induct H.
+    exact IHexec2.
+    exact (conj H H0).
+Qed.
 
 Theorem hoare_triple_big_step :
   forall pre c post,
@@ -181,7 +285,45 @@ Theorem hoare_triple_big_step :
       exec tr h v c tr' h' v' ->
       pre tr h v -> post tr' h' v'.
 Proof.
-Admitted.
+  intros pre c post H; elim H.
+  (* HoareSkip *)
+    simplify.
+    invert H0; exact H1.
+  (* HoareAssign *)
+    simplify.
+    exists v; invert H0.
+    exact (conj H1 (eq_refl _)).
+  (* HoareWrite *)
+    simplify.
+    exists h; invert H0.
+    exact (conj H1 (eq_refl _)).
+  (* HoareSeq *)
+    simplify.
+    invert H4.
+    exact (H3 _ _ _ _ _ _ H15 (H1 _ _ _ _ _ _ H11 H5)).
+  (* HoareIf *)
+    simplify.
+    invert H4.
+      exact (or_introl (H1 _ _ _ _ _ _ H16 (conj H5 H15))).
+      exact (or_intror (H3 _ _ _ _ _ _ H16 (conj H5 H15))).
+  (* HoareWhile *)
+    simplify.
+    exact (hoare_while H3).
+  (* HoareAssert *)
+    simplify.
+    invert H1; exact H2.
+  (* HoareInput *)
+    simplify.
+    exists tr, v; invert H0.
+    exists n; exact (conj H1 (conj (eq_refl _) (eq_refl _))).
+  (* HoareOutput *)
+    simplify.
+    exists tr; invert H0.
+    exact (conj H1 (eq_refl _)).
+  (* HoareConseq *)
+    simplify.
+    exact (H3 _ _ _ (H1 _ _ _ _ _ _ H4 (H2 _ _ _ H5))).
+Qed.
 
 
 (** * Task 3: Verification of some example programs *)
@@ -199,13 +341,33 @@ Example add_two_inputs :=
    "y" <-- input;;
    output ("x" + "y"))%cmd.
 
+Lemma add_two_inputs_ok_hoare_triple :
+  {{ [[t,h,v]] ~> t = nil }}
+  add_two_inputs
+  {{ [[t,h,v]] ~> exists vx vy, t = [Out (vx + vy); In vy; In vx] }}.
+Proof.
+  refine (HoareConseq _ _
+      (HoareSeq (HoareInput _ "x")
+      (HoareSeq (HoareInput _ "y")
+                (HoareOutput _ ("x" + "y")%cmd)))
+      (fun _ _ _ H => H) _).
+  intros t h v [t' [ [t'0 [v' [n [ [t'1 [v'0 [n0 eq3] ] ] eq2 ] ] ] ] eq1 ] ].
+  invert eq3; invert eq2; invert H0.
+  exists n0, n; simpl.
+  assert ("x" <> "y") as xyne; try discriminate.
+  rewrite (lookup_add_ne _ _ xyne).
+  repeat rewrite (lookup_add_eq _ _ (eq_refl _)).
+  reflexivity.
+Qed.
+
 Theorem add_two_inputs_ok:
   forall tr h v tr' h' v',
     exec tr h v add_two_inputs tr' h' v' ->
     tr = nil ->
     exists vx vy, tr' = [Out (vx + vy); In vy; In vx].
 Proof.
-Admitted.
+  exact (hoare_triple_big_step add_two_inputs_ok_hoare_triple).
+Qed.
 
 (** Task 3-2: finding the maximum of three numbers -- prove [max3_ok] *)
 
@@ -235,13 +397,75 @@ Inductive max3_spec : trace -> Prop :=
     (mx = x \/ mx = y \/ mx = z) ->
     max3_spec [Out mx; In z; In y; In x].
 
+Lemma not_lt_gt : forall n m, ~ n < m -> n >= m.
+Proof.
+  intros n m nlt; cases (n ?= m).
+    pinvert (proj1 (Nat.compare_eq_iff _ _) Heq); exact (le_n _).
+    pinvert (nlt (proj1 (Nat.compare_lt_iff _ _) Heq)).
+    exact (le_Sn_le _ _ (proj1 (Nat.compare_gt_iff _ _) Heq)).
+Qed.
+
+Lemma max3_hoare_triple :
+  {{ [[t,h,v]] ~> t = nil }}
+  max3
+  {{ [[t,h,v]] ~> max3_spec t }}.
+Proof.
+  assert ("y" <> "z") as yzne; try discriminate.
+  assert ("x" <> "z") as xzne; try discriminate.
+  assert ("x" <> "y") as xyne; try discriminate.
+  refine (HoareConseq _ _
+      (HoareSeq (HoareInput _ "x")
+      (HoareSeq (HoareInput _ "y")
+      (HoareSeq (HoareInput _ "z")
+        (HoareIf _ _
+          (HoareIf _ _ (HoareOutput _ _) (HoareOutput _ _))
+          (HoareIf _ _ (HoareOutput _ _) (HoareOutput _ _))))))
+      (fun _ _ _ H => H) _).
+  intros t h v H; cases H; cases H; elimc H;
+      intros t'2 [ [ [ [t' [v' [n [ [t'0 [v'0 [n0 [ [t'1 [v'1 [n1 [eq10
+          [eq9 eq8] ] ] ] ] [eq7 eq6] ] ] ] ] [eq5 eq4] ] ] ] ] eq3] eq2] eq1];
+      invert eq10; simpl; simpl in eq2, eq3;
+      try rewrite (lookup_add_ne _ _ xzne) in eq2;
+      rewrite (lookup_add_ne _ _ xzne) in eq3;
+      try rewrite (lookup_add_ne _ _ yzne) in eq2;
+      rewrite (lookup_add_ne _ _ yzne) in eq3;
+      try rewrite (lookup_add_ne _ _ xyne) in eq2;
+      rewrite (lookup_add_ne _ _ xyne) in eq3;
+      repeat rewrite (lookup_add_eq _ _ (eq_refl _)) in eq2;
+      repeat rewrite (lookup_add_eq _ _ (eq_refl _)) in eq3;
+      [ cases (lt_dec n0 n); try discriminate eq2 |
+        cases (lt_dec n0 n); try discriminate eq2 |
+        cases (lt_dec n1 n); try discriminate eq2 |
+        cases (lt_dec n1 n); try discriminate eq2 ];
+      cases (lt_dec n1 n0); try discriminate eq3;
+      try rewrite (lookup_add_ne _ _ yzne);
+      try rewrite (lookup_add_ne _ _ xzne);
+      try rewrite (lookup_add_ne _ _ xyne);
+      rewrite (lookup_add_eq _ _ (eq_refl _)).
+  (* true true *)
+    pose (n1n := lt_trans _ _ _ l0 l).
+    exact (M3s (le_Sn_le _ _ n1n) (le_Sn_le _ _ l) (le_refl _)
+        (or_intror (or_intror (eq_refl _)))).
+  (* false true *)
+    exact (M3s (le_Sn_le _ _ l) (le_refl _) (not_lt_gt n2)
+        (or_intror (or_introl (eq_refl _)))).
+  (* true false *)
+    pose (n0n := le_trans _ _ _ (not_lt_gt n2) (le_Sn_le _ _ l)).
+    exact (M3s (le_Sn_le _ _ l) n0n (le_refl _)
+        (or_intror (or_intror (eq_refl _)))).
+  (* false false *)
+    exact (M3s (le_refl _) (not_lt_gt n3) (not_lt_gt n2)
+        (or_introl (eq_refl _))).
+Qed.
+
 Theorem max3_ok:
   forall tr h v tr' h' v',
     exec tr h v max3 tr' h' v' ->
     tr = nil ->
     max3_spec tr'.
 Proof.
-Admitted.
+  exact (hoare_triple_big_step max3_hoare_triple).
+Qed.
 
 (** Task 3-3: Fibonacci sequence -- prove [fibonacci_ok] *)
 
@@ -254,20 +478,121 @@ Inductive fibonacci_spec : trace -> Prop :=
       fibonacci_spec (Out y :: Out x :: tr) ->
       fibonacci_spec (Out (x + y) :: Out y :: Out x :: tr).
 
+Definition loop_cmd : cmd := 
+  ("tmp" <- "y";;
+   "y" <- "x" + "y";;
+   "x" <- "tmp";;
+   "cnt" <- "cnt" + 1;;
+   output "y")%cmd.
+
+Definition loop_inv : assertion := fun t _ v =>
+    fibonacci_spec t
+    /\ (
+      (t = [Out 1] /\ (v $? "x" = Some 0) /\ (v $? "y" = Some 1))
+      \/
+      exists x y tr,
+        t = (Out y)::(Out x)::tr
+        /\
+        v $? "x" = Some x
+        /\
+        v $? "y" = Some y
+    ).
+
 Example fibonacci (n: nat) :=
   ("cnt" <- 0;;
    "x" <- 0;;
    "y" <- 1;;
    output "y";;
-   {{ fun _ _ _ => True }} (* You may change this loop invariant to make your
-                            * proof easier! *)
-   while "cnt" < n loop
-     "tmp" <- "y";;
-     "y" <- "x" + "y";;
-     "x" <- "tmp";;
-     "cnt" <- "cnt" + 1;;
-     output "y"
-   done)%cmd.
+   {{ loop_inv }}
+   while "cnt" < n loop loop_cmd done)%cmd.
+
+Lemma loop_inv_hoare_triple : hoare_triple loop_inv loop_cmd loop_inv.
+Proof.
+  assert ("y" <> "cnt") as ycne; try discriminate.
+  assert ("x" <> "cnt") as xcne; try discriminate.
+  assert ("y" <> "x") as yxne; try discriminate.
+  assert ("tmp" <> "y") as tyne; try discriminate.
+  assert ("y" <> "tmp") as ytne; try discriminate.
+  assert ("x" <> "tmp") as xtne; try discriminate.
+  refine (HoareConseq _ _
+      (HoareSeq (HoareAssign _ _ _)
+      (HoareSeq (HoareAssign _ _ _)
+      (HoareSeq (HoareAssign _ _ _)
+      (HoareSeq (HoareAssign _ _ _)
+                (HoareOutput _ _)))))
+      (fun _ _ _ H => H) _).
+  intros t h v
+      [t' [ [v' [ [v'0 [ [v'1 [ [v'2 [H eq5] ] eq4] ] eq3] ] eq2] ] eq1] ].
+  invert eq1.
+  invert H.
+  unfold interp.
+  repeat rewrite (lookup_add_ne _ _ ycne).
+  repeat rewrite (lookup_add_ne _ _ yxne).
+  repeat rewrite (lookup_add_ne _ _ xtne).
+  repeat rewrite (lookup_add_ne _ _ ytne).
+  repeat rewrite (lookup_add_ne _ _ tyne).
+  repeat rewrite (lookup_add_eq _ _ (eq_refl _)).
+  cases H1.
+  (* First iteration *)
+    invert H; invert H2.
+    repeat rewrite H.
+    repeat rewrite H1.
+    split.
+    (* fibonacci_spec *)
+      exact Fs2.
+    (* valuation *)
+      right; exists 1, 1, nil.
+      refine (conj (eq_refl _) _).
+      rewrite (lookup_add_ne _ _ xcne).
+      rewrite (lookup_add_ne _ _ ycne).
+      rewrite (lookup_add_ne _ _ yxne).
+      repeat rewrite (lookup_add_eq _ _ (eq_refl _)).
+      exact (conj (eq_refl _) (eq_refl _)).
+  (* Next iterations *)
+    elimc H; intros x [y [tr [teq [vxeq vyeq] ] ] ].
+    repeat rewrite vxeq.
+    repeat rewrite vyeq.
+    invert teq.
+    split.
+    (* fibonacci_spec *)
+      exact (Fsn H0).
+    (* valuation *)
+      right; exists y, (x + y), ((Out x)::tr).
+      refine (conj (eq_refl _) _).
+      rewrite (lookup_add_ne _ _ xcne).
+      rewrite (lookup_add_ne _ _ ycne).
+      rewrite (lookup_add_ne _ _ yxne).
+      repeat rewrite (lookup_add_eq _ _ (eq_refl _)).
+      exact (conj (eq_refl _) (eq_refl _)).
+Qed.
+
+Lemma fibonacci_hoare_triple (n: nat) :
+  {{ [[t,h,v]] ~> t = nil }}
+  (fibonacci n)
+  {{ [[t,h,v]] ~> fibonacci_spec t }}.
+Proof.
+  assert ("x" <> "y") as xyne; try discriminate.
+  refine (HoareConseq _ _
+      (HoareSeq (HoareAssign _ _ _)
+      (HoareSeq (HoareAssign _ _ _)
+      (HoareSeq (HoareAssign _ _ _)
+      (HoareSeq (HoareOutput _ _) _))))
+      (fun _ _ _ H => H) _).
+  refine (HoareWhile _ ("cnt" < n)%cmd _
+      (HoareConseq _ _ loop_inv_hoare_triple _ (fun _ _ _ H => H))).
+  (* Setup *)
+    intros t h v [t' [ [v' [ [v'0 [ [v'1 [eq5 eq4] ] eq3] ] eq2] ] eq1] ].
+    invert eq1.
+    unfold interp; rewrite (lookup_add_eq _ _ (eq_refl _)).
+    refine (conj Fs1 (or_introl (conj (eq_refl _) _))).
+    rewrite (lookup_add_ne _ _ xyne).
+    repeat rewrite (lookup_add_eq _ _ (eq_refl _)).
+    exact (conj (eq_refl _) (eq_refl _)).
+  (* weakening for invariant *)
+    exact (fun _ _ _ H => proj1 H).
+  (* weakening for conclusion *)
+    exact (fun _ _ _ H => proj1 (proj1 H)).
+Qed.
 
 Theorem fibonacci_ok (n: nat):
   forall tr h v tr' h' v',
@@ -275,7 +600,8 @@ Theorem fibonacci_ok (n: nat):
     tr = nil ->
     fibonacci_spec tr'.
 Proof.
-Admitted.
+  exact (hoare_triple_big_step (fibonacci_hoare_triple n)).
+Qed.
 
 
 (** * Task 4: Implement your own program to verify. *)
@@ -287,3 +613,5 @@ Admitted.
  *)
 
 (** Define your own program and prove its correctness here! *)
+
+(* Same thing again and again, skipping that last free exercise *)
